\documentclass{article}

\usepackage{bbm}
\usepackage{amsmath}
\usepackage{amssymb}
\date{\today}

\begin{document}
	Factorisons $\frac{n^2+n}{3}$ par $n$:
	\[\frac{n^2+n}{3}=\frac{n(n+1)}{3}\]
	Calculons $\frac{2}{3}\times$ la somme des n premiers entiers :
	\[
		\frac{2}{3}\displaystyle\sum^n_{k=0}k=\displaystyle\sum^n_{k=0}\frac{2}{3}k=\frac{2n(n+1)}{3\times 2}=\frac{n(n+1)}{3}
	\]
	C'est exactement :
	\[\frac{n(n+1)}{3}\]
	Or, nous savons que :
	\[\displaystyle\sum^n_{k=0}u_k=\frac{n(n+1)}{3}\]
	Ainsi :
	\[\frac{n(n+1)}{3}=\displaystyle\sum^n_{k=0}\frac{2}{3}k=\displaystyle\sum^n_{k=0}u_k\]
	Par identification :
	\[u_n = \frac{2}{3}n\]
\end{document}

